metatheory/typeSoundInvariantsScript.sml
@@ -21,15 +21,28 @@ val _ = type_abbrev( "tenvS" , ``: (num, t) env``);
 (* Constructor type environments keyed by constructor namd and type *)
 val _ = type_abbrev( "tenvCT" , ``: (( conN id # tid_or_exn), ( tvarN list # t list)) env``);
 
+(*val same_module : id conN -> tid_or_exn -> bool*)
+ val _ = Define `
+ (same_module (Short x) _ = T)
+/\
+(same_module (Long mn1 x) (TypeId (Long mn2 y)) = (mn1 = mn2))
+/\
+(same_module _ TypeExn = T)
+/\
+(same_module _ _ = F)`;
+
+
+(*val tenvC_ok : tenvC -> bool*)
 val _ = Define `
  (tenvC_ok tenvC =  
-(EVERY (\ (cn,(tvs,ts,tn)) .  EVERY (check_freevars( 0) tvs) ts) tenvC))`;
+(EVERY (\ (cn,(tvs,ts,tn)) .  same_module cn tn /\ EVERY (check_freevars( 0) tvs) ts) tenvC))`;
 
 
+(*val tenvCT_ok : tenvCT -> bool*)
 val _ = Define `
  (tenvCT_ok tenvCT =  
 (
-  (*all_distinct (List.map fst tenvCT) &&*)EVERY (\ ((cn,tn),(tvs,ts)) .  EVERY (check_freevars( 0) tvs) ts) tenvCT))`;
+  (*all_distinct (List.map fst tenvCT) &&*)EVERY (\ ((cn,tn),(tvs,ts)) .  same_module cn tn /\ EVERY (check_freevars( 0) tvs) ts) tenvCT))`;
 
 
 (* Check that a constructor type environment is consistent with a runtime type
